SpecDefines.v
@@ -14,7 +14,7 @@
  * limitations under the License.
  *)
 
-From Stdlib Require Import String List ZArith Zmod Psatz.
+From Stdlib Require Import String List ZArith Zmod Psatz Bool.
 From Guru Require Import Library Syntax Notations Composition.
 From Cheriot Require Import Fifo.
 
@@ -77,6 +77,7 @@ Definition FullCapSz := Eval compute in (kindSize Cap + Xlen).
 Definition NumBytesFullCapSz := Eval compute in (FullCapSz / 8).
 Definition LgNumBytesFullCapSz := Eval compute in Z.log2_up NumBytesFullCapSz.
 Definition LgLgNumBytesFullCapSz := Eval compute in Z.log2_up (LgNumBytesFullCapSz + 1).
+Definition TagAddrWidth : Z := Eval compute in (AddrSz - LgNumBytesFullCapSz).
 
 Definition isCompressed ty (inst: ty Inst) : Expr ty Bool := Not (isAllOnes (TruncLsb (InstSz-2) 2 #inst)).
 Definition getCd ty (inst: ty Inst) : Expr ty (Bit RegIdxSz) := #inst`[11:7].
@@ -1044,3 +1045,124 @@ Definition coreTree (memTree : Tree Elem) (fetchCapacity deferredCapacity : nat)
     fetchTree fetchCapacity ;
     deferredTree deferredCapacity
   ].
+
+Record MemConfig := {
+  binary                  : list Z ;
+  mainMemStartAddr        : Z ;
+  mainMemSize             : nat ;
+  mainMemBoundProof       : Is_true (mainMemStartAddr + Z.of_nat mainMemSize <? Z.shiftl 1 Xlen)%Z ;
+  lgMainMemSize_ge_binary : Is_true (length binary <=? mainMemSize)%nat ;
+
+  (* Heap & Revocation Configuration *)
+  heapStartAddr           : Z ;
+  heapSize                : nat ;
+  lgRevGranularity        : Z ;
+  revTableStartAddr       : Z ;
+
+  (* Proofs *)
+  heap_in_mainMem_proof :
+    Is_true ((mainMemStartAddr <=? heapStartAddr) &&
+             (heapStartAddr + Z.of_nat heapSize <=? mainMemStartAddr + Z.of_nat mainMemSize))%Z ;
+  revTable_in_mainMem_proof :
+    Is_true ((mainMemStartAddr <=? revTableStartAddr) &&
+             (revTableStartAddr + Z.shiftr (Z.of_nat heapSize) (lgRevGranularity + 3)
+              <=? mainMemStartAddr + Z.of_nat mainMemSize))%Z ;
+  revTable_heap_disjoint_proof :
+    Is_true ((revTableStartAddr + Z.shiftr (Z.of_nat heapSize) (lgRevGranularity + 3) <=? heapStartAddr) ||
+             (heapStartAddr + Z.of_nat heapSize <=? revTableStartAddr))%Z
+}.
+
+Section SpecMemoryLayout.
+  Variable config : MemConfig.
+
+  Definition fixedBinary : list (bits 8) :=
+    map (fun v => bits.of_Z 8 v) config.(binary).
+
+  Definition heapEndAddr :=
+    config.(heapStartAddr) + Z.of_nat config.(heapSize).
+
+  Definition paddedBinary :=
+    (fixedBinary ++ List.repeat (bits.of_Z 8 0) (config.(mainMemSize) - length config.(binary)))%list.
+
+  Lemma paddedBinary_length :
+    length paddedBinary = config.(mainMemSize).
+  Proof.
+    unfold paddedBinary, fixedBinary.
+    rewrite length_app.
+    rewrite repeat_length.
+    rewrite length_map.
+    pose proof config.(lgMainMemSize_ge_binary) as H.
+    apply Is_true_eq_true in H.
+    rewrite Nat.leb_le in H.
+    lia.
+  Qed.
+
+  Definition tagsStartAddr := Z.shiftr (config.(mainMemStartAddr) + NumBytesFullCapSz - 1) LgNumBytesFullCapSz.
+  Definition tagsEndAddr   := Z.shiftr (config.(mainMemStartAddr) + Z.of_nat config.(mainMemSize)) LgNumBytesFullCapSz.
+  Definition tagsSize : nat := Z.to_nat (tagsEndAddr - tagsStartAddr).
+
+  Definition isMemAddr {ty: Kind -> Type} (a : Expr ty Addr) : Expr ty Bool :=
+    Sge a (Const ty Addr (bits.of_Z Xlen config.(mainMemStartAddr))).
+
+  Definition isTagsAddr {ty: Kind -> Type} (a : Expr ty (Bit TagAddrWidth)) : Expr ty Bool :=
+    Sge a (Const ty (Bit TagAddrWidth) (bits.of_Z TagAddrWidth tagsStartAddr)).
+
+  Definition isHeapAddr {ty: Kind -> Type} (a : Expr ty (Bit (AddrSz + 1))) : Expr ty Bool :=
+    And [ Sge a (Const ty (Bit (AddrSz + 1)) (bits.of_Z (AddrSz + 1) config.(heapStartAddr))) ;
+          Slt a (Const ty (Bit (AddrSz + 1)) (bits.of_Z (AddrSz + 1) heapEndAddr)) ].
+
+  Definition specMemTree : Tree Elem :=
+    Node "mem" [
+      Leaf "mainMem" (EReg {| regKind := Array config.(mainMemSize) (Bit 8);
+                              regInit := Some (Build_SameTuple (tupleElems := paddedBinary)
+                                                 (Is_true_Nat_eq_implies paddedBinary_length)) |}) ;
+      Leaf "tags" (EReg {| regKind := Array tagsSize Bool;
+                           regInit := Some (Build_SameTuple (tupleElems := List.repeat false tagsSize)
+                                               (Is_true_Nat_eq_implies (repeat_length false tagsSize))) |})
+    ].
+
+  Definition specTree : Tree Elem :=
+    Node "core" [
+      rfTree ;
+      specMemTree
+    ].
+
+  Definition RevBitLookup := STRUCT_TYPE {
+    "isHeap"      :: Bool ;
+    "revByteAddr" :: Addr ;
+    "bitInByte"   :: Bit 3
+  }.
+
+  Section RevBits.
+    Variable ty : Kind -> Type.
+
+    Definition computeRevBitAddr (base : Expr ty (Bit (AddrSz + 1))) : LetExpr ty RevBitLookup.
+      refine (
+        LetE is_heap : Bool <- isHeapAddr base ;
+        LetE heapOffset : Bit (AddrSz + 1) <-
+          Sub base (Const ty (Bit (AddrSz + 1)) (bits.of_Z (AddrSz + 1) config.(heapStartAddr))) ;
+        LetE castHeapOffset <- castBits _ #heapOffset ;
+        LetE totalBitIdx : Bit ((AddrSz + 1) - config.(lgRevGranularity)) <-
+          TruncMsb ((AddrSz + 1) - config.(lgRevGranularity)) config.(lgRevGranularity) #castHeapOffset ;
+        LetE castTotalBitIdx <- castBits _ #totalBitIdx ;
+        LetE byteIdxInTable : Bit (((AddrSz + 1) - config.(lgRevGranularity)) - 3) <-
+          TruncMsb (((AddrSz + 1) - config.(lgRevGranularity)) - 3) 3 #castTotalBitIdx ;
+        LetE byteIdxExt : Bit AddrSz <- castBits _ (ZeroExtendTo AddrSz #byteIdxInTable) ;
+        LetE revByteAddr : Addr <-
+          Add [ Const ty Addr (bits.of_Z Xlen config.(revTableStartAddr)) ; #byteIdxExt ] ;
+        LetE bitInByte : Bit 3 <-
+          TruncLsb (((AddrSz + 1) - config.(lgRevGranularity)) - 3) 3 #castTotalBitIdx ;
+        @RetE ty RevBitLookup (STRUCT {
+          "isHeap"      ::= #is_heap ;
+          "revByteAddr" ::= #revByteAddr ;
+          "bitInByte"   ::= #bitInByte
+        })
+      )%guru; abstract lia.
+    Defined.
+  End RevBits.
+End SpecMemoryLayout.
+
+Definition extractRevBit {ty : Kind -> Type} (lookup : ty RevBitLookup) (byteVal : Expr ty (Bit 8)) : Expr ty Bool :=
+  ITE (##lookup`"isHeap")
+      (ReadArray (FromBit (Array 8 Bool) byteVal) (##lookup`"bitInByte"))
+      (ConstBool false).
