SpecFetchMemory.v
@@ -1,0 +1,205 @@
+(*
+ * Copyright 2026 Google LLC
+ *
+ * Licensed under the Apache License, Version 2.0 (the "License");
+ * you may not use this file except in compliance with the License.
+ * You may obtain a copy of the License at
+ *
+ *     https://www.apache.org/licenses/LICENSE-2.0
+ *
+ * Unless required by applicable law or agreed to in writing, software
+ * distributed under the License is distributed on an "AS IS" BASIS,
+ * WITHOUT WARRANTIES OR CONDITIONS OF ANY KIND, either express or implied.
+ * See the License for the specific language governing permissions and
+ * limitations under the License.
+ *)
+
+From Stdlib Require Import String List ZArith Zmod Psatz Bool.
+From Guru Require Import Syntax Notations Semantics Library Composition.
+From Cheriot Require Import SpecDefines Decoder FunctionalUnits Alu.
+
+Set Implicit Arguments.
+Unset Strict Implicit.
+Set Asymmetric Patterns.
+
+Import ListNotations.
+Local Open Scope Z_scope.
+Local Open Scope string_scope.
+Local Open Scope guru_scope.
+
+Section SpecFetchMemory.
+  Variable config : MemConfig.
+  Variable ty : Kind -> Type.
+
+  Local Notation memTree := (specMemTree config).
+  Local Notation tree := (specTree config).
+  Local Notation isMemAddr := (isMemAddr config).
+  Local Notation isTagsAddr := (isTagsAddr config).
+  Local Notation isHeapAddr := (isHeapAddr config).
+  Local Notation tagsStartAddr := (tagsStartAddr config).
+  Local Notation tagsSize := (tagsSize config).
+
+  Definition np_rf : NodePath tree :=
+    getNodePath tree "core.rf".
+
+  Definition np_mem : NodePath tree :=
+    getNodePath tree "core.mem".
+
+  Local Notation computeRevBitAddr := (computeRevBitAddr config).
+
+  (* =========================================================================
+   * Revocation Bit Helper (Combinational Action on specMemTree)
+   * ========================================================================= *)
+  Definition readRevBit (base : Expr ty (Bit (AddrSz + 1))) : Action ty memTree Bool :=
+    LetL lookup  : RevBitLookup <- computeRevBitAddr base ;
+    Let  offset  <- getMemOffset config.(mainMemStartAddr) (Z.of_nat config.(mainMemSize)) ##lookup`"revByteAddr" ;
+    RegRead memVal <- "mem.mainMem" in memTree ;
+    Let  byteVal : Bit 8 <- ReadArray #memVal #offset ;
+    Let  revBit  : Bool  <- extractRevBit lookup #byteVal ;
+    Return #revBit.
+
+  (* =========================================================================
+   * 1. specFetch (Atomic Combinational Fetch)
+   * ========================================================================= *)
+  Definition specFetch : Action ty tree FetchOut :=
+    LetA pcc : FullECapWithTag <- liftAction np_rf (readRegsList gprPathsWithKind ($0 : Expr ty (Bit RegIdxSzReal))) ;
+    Let offset <- getMemOffset config.(mainMemStartAddr) (Z.of_nat config.(mainMemSize)) ##pcc`"addr" ;
+    LetA rawInst : Inst <- liftAction np_mem (
+      RegRead memVal <- "mem.mainMem" in memTree ;
+      Let instBytes : Array (Z.to_nat (InstSz / 8)) (Bit 8) <- slice #memVal #offset (Z.to_nat (InstSz / 8)) ;
+      Return (ToBit #instBytes)
+    ) ;
+
+    (* Fetch Exception Checks *)
+    Let isComp       : Bool <- isCompressed rawInst ;
+    Let instBytesLen : Addr <- ITE #isComp $(CompInstSz / 8) $(InstSz / 8) ;
+    Let tagExc       : Bool <- Not ##pcc`"tag" ;
+    Let sealExc      : Bool <- isNotZero (##pcc`"ecap"`"oType") ;
+    Let permExc      : Bool <- Not (##pcc`"ecap"`"perms"`"EX") ;
+    Let boundsExc    : Bool <- Or [
+      Slt (ZeroExtendTo (AddrSz + 2) ##pcc`"addr") (ZeroExtendTo (AddrSz + 2) ##pcc`"ecap"`"base") ;
+      Sgt (ZeroExtendTo (AddrSz + 2) (Add [ ##pcc`"addr" ; #instBytesLen ])) (##pcc`"ecap"`"top")
+    ] ;
+
+    Let fetchOut : FetchOut <- STRUCT {
+      "pcc"      ::= #pcc ;
+      "inst"     ::= #rawInst ;
+      "fetchExc" ::= STRUCT {
+        "tag"    ::= #tagExc ;
+        "seal"   ::= #sealExc ;
+        "perm"   ::= #permExc ;
+        "bounds" ::= #boundsExc
+      }
+    } ;
+    Return #fetchOut.
+
+  (* =========================================================================
+   * 2. specExecuteDeferredReq (Single Deferred Request execution)
+   * ========================================================================= *)
+  Definition specExecuteDeferredReq (req : ty DeferredReq) : Action ty tree (Bit 0) :=
+    Let  dstIdx : Bit RegIdxSz   <- ##req`"dstIdx" ;
+    Let  addr   : Addr           <- ##req`"addr" ;
+    Let  op     : DeferredUnion  <- ##req`"op" ;
+
+    If (#op `? "Mem") Then (
+      Let memPayload : MemPayload        <- #op `! "Mem" ;
+      Let memSize    : Bit LgLgNumBytesFullCapSz <- ##memPayload`"memSize" ;
+      Let memOp      : LoadOrStoreKind   <- ##memPayload`"memOp" ;
+      Let isCap      : Bool              <- Eq #memSize $LgNumBytesFullCapSz ;
+
+      Let offset     <- getMemOffset config.(mainMemStartAddr) (Z.of_nat config.(mainMemSize)) #addr ;
+      Let tagAddr    : Bit TagAddrWidth  <- TruncMsb TagAddrWidth LgNumBytesFullCapSz #addr ;
+      Let tagOffset  <- getMemOffset tagsStartAddr (Z.of_nat tagsSize) #tagAddr ;
+
+      If (#memOp `? "Store") Then (
+        Let stCapVal   : FullCapWithTag <- #memOp `! "Store" ;
+        Let stTag      : Bool           <- And [ #isCap ; ##stCapVal`"tag" ] ;
+        Let rawData    : Bit FullCapSz  <-
+          ITE #isCap
+              {< ToBit ##stCapVal`"cap", ##stCapVal`"addr" >}
+              (ZeroExtendTo FullCapSz ##stCapVal`"addr") ;
+        Let num_bytes  : Bit (LgNumBytesFullCapSz + 1) <- Sll $1 #memSize ;
+
+        Act (liftAction np_mem (
+          RegRead memVal  <- "mem.mainMem" in memTree ;
+          RegRead tagsVal <- "mem.tags"    in memTree ;
+          LetL updatedMem : Array config.(mainMemSize) (Bit 8) <-
+            updSlice #memVal #offset (FromBit (Array (Z.to_nat NumBytesFullCapSz) (Bit 8)) #rawData) #num_bytes ;
+          RegWrite "mem.mainMem" in memTree <- #updatedMem ;
+          RegWrite "mem.tags" in memTree <- UpdateArray #tagsVal #tagOffset #stTag ;
+          Retv
+        )) ;
+        Retv
+      ) Else (
+        (* Load Operation *)
+        Let  ldOpVal    : LoadOp <- #memOp `! "Load" ;
+        Let  isUnsigned : Bool   <- ##ldOpVal`"isUnsigned" ;
+        LetA rawBits    : Bit FullCapSz <-
+          liftAction np_mem (
+            RegRead memVal <- "mem.mainMem" in memTree ;
+            Let dataBytes : Array (Z.to_nat NumBytesFullCapSz) (Bit 8) <- slice #memVal #offset (Z.to_nat NumBytesFullCapSz) ;
+            Return (ToBit #dataBytes)
+          ) ;
+        LetA rawTag : Bool <-
+          liftAction np_mem (
+            RegRead tagsVal <- "mem.tags" in memTree ;
+            Let rawTag : Bool <- ReadArray #tagsVal #tagOffset ;
+            Return #rawTag
+          ) ;
+        Let rawDataLsb : Addr          <- TruncLsb Xlen Xlen #rawBits ;
+        Let rawCap     : Cap           <- FromBit Cap (TruncMsb Xlen Xlen #rawBits) ;
+
+        If #isCap Then (
+          LetL ldECap : ECap <- DecodeCap rawCap rawDataLsb ;
+          LetIf finalTag : Bool <-
+            If #rawTag Then (
+              LetA revBit : Bool <- liftAction np_mem (readRevBit (##ldECap`"base")) ;
+              Return (Not #revBit)
+            ) Else (
+              Return (ConstBool false)
+            ) ;
+          Let dstVal : FullECapWithTag <- STRUCT {
+            "tag"  ::= #finalTag ;
+            "ecap" ::= #ldECap ;
+            "addr" ::= #rawDataLsb
+          } ;
+          If (isNotZero #dstIdx) Then (
+            liftAction np_rf (writeRegsList gprPathsWithKind #dstIdx #dstVal)
+          ) ;
+          Retv
+        ) Else (
+          Let rawBytes   : Array (Z.to_nat NumBytesXlen) (Bit 8) <-
+            FromBit (Array (Z.to_nat NumBytesXlen) (Bit 8)) #rawDataLsb ;
+          Let memSzBytes : Bit (LgNumBytesFullCapSz + 1) <- Sll $1 #memSize ;
+          Let readBits   : Bit Xlen <- ToBit (
+            ITE #isUnsigned
+                (ArrayZeroExtend #memSzBytes #rawBytes)
+                (ArraySignExtend #memSzBytes #rawBytes)
+          ) ;
+          Let dstVal : FullECapWithTag <- STRUCT {
+            "tag"  ::= Const ty Bool false ;
+            "ecap" ::= Const ty ECap (getDefault _) ;
+            "addr" ::= #readBits
+          } ;
+          If (isNotZero #dstIdx) Then (
+            liftAction np_rf (writeRegsList gprPathsWithKind #dstIdx #dstVal)
+          ) ;
+          Retv
+        ) ;
+        Retv
+      ) ;
+      Retv
+    ) ;
+    Retv.
+
+  (* =========================================================================
+   * 3. specExecuteDeferred (Executing Option DeferredReq)
+   * ========================================================================= *)
+  Definition specExecuteDeferred (reqOpt : ty (Option DeferredReq)) : Action ty tree (Bit 0) :=
+    If (##reqOpt `? "Some") Then (
+      Let req : DeferredReq <- ##reqOpt `! "Some" ;
+      specExecuteDeferredReq req
+    ) ;
+    Retv.
+
+End SpecFetchMemory.
